% Corollary 1.21
\section*{Corollary 1.21}
$(-1)(-1) = 1$.
\begin{proof}
  %We apply Proposition 1.20 with $m = n = 1$.
  \begin{align*}
    (-1)(-1) & = 1 \cdot 1 &  & \text{(Proposition 1.20 with $m = n = 1$)} \\
             & = 1         &  & \text{(Axiom 1.3)}
  \end{align*}
\end{proof}

% Corollary 4.20
\section*{Corollary 4.20:}
For $1 \leq m \leq k$,
$\binom{k+1}{m} = \binom{k}{m-1} + \binom{k}{m}$

% Corollary 4.22
\section*{Corollary 4.22:}
For $k \in \mathbb{Z}_{\geq 0}$,
$\displaystyle\sum_{m=0}^{k} \binom{k}{m} = 2^k$